sorting.v
@@ -1,0 +1,272 @@
+(**************************************************************)
+(*   Copyright Dominique Larchey-Wendling [*]                 *)
+(*                                                            *)
+(*                             [*] Affiliation LORIA -- CNRS  *)
+(**************************************************************)
+(*      This file is distributed under the terms of the       *)
+(*         CeCILL v2 FREE SOFTWARE LICENSE AGREEMENT          *)
+(**************************************************************)
+
+Require Import List Arith Lia Wellfounded.
+
+Require Import bt env fun_defs.
+
+Set Implicit Arguments.
+
+Local Notation "e ⇢ x" := (@get_env _ _ e x).
+Local Notation "e ⦃  x ⇠ v ⦄" := (@set_env _ _ Var_eq_dec e x v).
+
+Section measure_rect.
+
+  Variables (X : Type) (m : X -> nat) (P : X -> Type)
+            (HP : forall x, (forall y, m y < m x -> P y) -> P x).
+
+  Theorem measure_rect : forall x, P x.
+  Proof.
+    apply (@well_founded_induction_type _ (fun x y => m x < m y)); auto.
+    apply wf_inverse_image, lt_wf.
+  Qed.
+
+End measure_rect.
+
+Tactic Notation "induction" "on" hyp(x) "as" ident(IH) "with" "measure" uconstr(f) :=
+  induction x as [ x IH ] using (@measure_rect _ (fun x => f)). 
+
+Section measure_rect2.
+
+  Variables (X Y : Type) (m : X -> Y -> nat) (P : X -> Y -> Type)
+            (HP : forall x y, (forall x' y', m x' y' < m x y -> P x' y') -> P x y).
+
+  Let Q (c : X*Y) := P (fst c) (snd c).
+
+  Theorem measure_rect2 : forall x y, P x y.
+  Proof.
+    intros x y.
+    change (Q (x,y)).
+    generalize (x,y); clear x y; intros c.
+    induction on c as IHc with measure (m (fst c) (snd c)).
+    destruct c as (x,y); simpl in *.
+    apply HP.
+    intros x' y'; simpl; apply (IHc (x',y')).
+  Qed. 
+
+End measure_rect2.
+
+Tactic Notation "induction" "on" hyp(x) hyp(y) "as" ident(IH) "with" "measure" uconstr(f) :=
+  revert x y; apply measure_rect2 with (m := fun x y => f); intros x y IH.
+
+Section sorting.
+
+  Variables (u x y z : Var) (Hxy : x <> y) (Hxz : x <> z) (Hyz : y <> z) (Hux : u <> x) (Huy : u <> y) (Huz : u <> z).
+
+  Variable (p_split p_merge p_merge_sort p_cmp p_leq : Fun).
+
+  Variable (param : Fun -> Var)     
+           (body : Fun -> fun_expr).
+
+  Notation "f // s ~~> v" := (fun_sem param body f s v).
+
+  Definition fe_cmp := 
+    MATCH £u WITH
+        ø   ⇒ ø 
+     OR x#y ⇒ MATCH £x WITH
+          ø   ⇒ MATCH £y WITH
+            ø   ⇒ ø
+         OR x#x ⇒ ø#ø
+       OR u#x ⇒ MATCH £y WITH
+            ø   ⇒ ø#(ø#ø)
+         OR z#y ⇒ MATCH CALL p_cmp ON (£u#£z) WITH
+              ø   ⇒ CALL p_cmp ON (£x#£y)
+           OR u#x ⇒ £u#£x.
+
+  Hypothesis (Hparam_cmp : param p_cmp = u) (Hbody_cmp : body p_cmp = fe_cmp).
+
+  Fact fe_cmp_spec f e a b : f // e ~~> ⟨a,b⟩ -> CALL p_cmp ON f // e ~~> bt_compare a b.
+  Proof.
+    revert b e f; induction a as [ | a1 H1 a2 H2 ]; intros [ | b1 b2 ] e f H;
+      constructor 7 with (1 := H); rewrite Hbody_cmp, Hparam_cmp; unfold fe_cmp.
+    + constructor 5 with ω ω.
+      1: apply fs_var; rew env.
+      constructor 4.
+      1: apply fs_var; rew env.
+      constructor 4.
+      1: apply fs_var; rew env.
+      constructor 2.
+    + constructor 5 with ω ⟨b1,b2⟩.
+      1: apply fs_var; rew env.
+      constructor 4.
+      1: apply fs_var; rew env.
+      constructor 5 with b1 b2.
+      1: apply fs_var; rew env.
+      constructor 3; constructor 2.
+    + constructor 5 with ⟨a1,a2⟩ ω.
+      1: apply fs_var; rew env.
+      constructor 5 with a1 a2.
+      1: apply fs_var; rew env.
+      constructor 4.
+      1: apply fs_var; rew env.
+      repeat constructor 3; constructor 2.
+    + constructor 5 with ⟨a1,a2⟩ ⟨b1,b2⟩.
+      1: apply fs_var; rew env.
+      constructor 5 with a1 a2.
+      1: apply fs_var; rew env.
+      constructor 5 with b1 b2.
+      1: apply fs_var; rew env.
+      match goal with |- _ // ?e ~~> _ => set (e' := e) end. 
+      specialize (H1 b1 e' (£u#£z)).
+      simpl.
+      destruct (bt_compare a1 b1) as [ | x1 x2 ].
+      * constructor 4.
+        1: apply H1; unfold e'; constructor 3; apply fs_var; rew env.
+        apply H2; constructor 3; unfold e'; apply fs_var; rew env.
+      * constructor 5 with x1 x2.
+        1:apply H1; unfold e'; constructor 3; apply fs_var; rew env.
+        constructor 3; apply fs_var; rew env.
+  Qed.
+
+  Definition fe_leq :=
+    MATCH CALL p_cmp ON £u WITH
+        ø   ⇒ ø#ø
+     OR x#x ⇒ MATCH £x WITH
+          ø   ⇒ ø#ø
+       OR x#x ⇒ ø.
+
+  Hypothesis (Hparam_leq : param p_leq = u) (Hbody_leq : body p_leq = fe_leq).
+
+  Fact fe_leq_spec f e a b : f // e ~~> ⟨a,b⟩ -> CALL p_leq ON f // e ~~> bt_leq a b.
+  Proof.
+    intros H.
+    constructor 7 with (1 := H); rewrite Hbody_leq, Hparam_leq; unfold fe_leq.
+    generalize (@fe_cmp_spec £u (e⦃u⇠⟨a,b⟩⦄) a b) (bt_compare_3 a b).
+    unfold bt_leq. 
+    intros H1 [ H2 | [ H2 | H2 ] ].
+    + constructor 4.
+      * rewrite <- H2; apply H1, fs_var; rew env.
+      * rewrite H2; constructor 3; constructor 2.
+    + constructor 5 with ω ω.
+      * rewrite <- H2; apply H1, fs_var; rew env.
+      * constructor 4.
+        1: apply fs_var; rew env.
+        rewrite H2; constructor 3; constructor 2.
+    + constructor 5 with ω ⟨ω,ω⟩.
+      * rewrite <- H2.
+        apply fe_cmp_spec, fs_var; rew env.
+      * rewrite H2.
+        constructor 5 with ω ω.
+        1: apply fs_var; rew env.
+        constructor 2.
+  Qed.
+
+  Definition fe_split :=
+    MATCH £u WITH
+        ø   ⇒ ø#ø
+     OR x#u ⇒ MATCH £u WITH
+          ø   ⇒ (£x#ø)#ø
+       OR y#u ⇒ MATCH CALL p_split ON £u WITH
+            ø   ⇒ ø#ø
+         OR u#z ⇒ (£x#£u)#(£y#£z).
+
+  Hypothesis (Hparam_split : param p_split = u) (Hbody_split : body p_split = fe_split).
+
+  Fact fe_split_spec f e l : f // e ~~> l -> CALL p_split ON f // e ~~> bt_split l.
+  Proof.
+    revert f e.
+    induction on l as IHl with measure (bt_length l); intros f e H.
+    constructor 7 with (1 := H); rewrite Hbody_split, Hparam_split; unfold fe_split.
+    destruct l as [ | t1 [ | t2 l ] ].
+    + constructor 4.
+      1: apply fs_var; rew env.
+      simpl; constructor 3; constructor 2.
+    + constructor 5 with t1 ω.
+      1: apply fs_var; rew env.
+      simpl; constructor 4.
+      1: apply fs_var; rew env.
+      repeat constructor 3; try constructor 2.
+      apply fs_var; rew env.
+    + constructor 5 with t1 ⟨t2,l⟩.
+      1: apply fs_var; rew env.
+      constructor 5 with t2 l.
+      1: apply fs_var; rew env.
+      specialize (IHl l); simpl.
+      destruct (bt_split l) as [ | l1 l2 ].
+      * constructor 4. 
+        - apply IHl; simpl; try lia.
+          apply fs_var; rew env.
+        - constructor 3; constructor 2.
+      * constructor 5 with l1 l2.
+        - apply IHl; simpl; try lia.
+          apply fs_var; rew env.
+        - constructor 3; constructor 3; apply fs_var; rew env.
+  Qed.
+
+(*
+  Fixpoint bt_merge_rec n l m :=
+  match n with 
+    | 0   => ω
+    | S n => match l, m with 
+               | ω    , _       => m
+               | _    , ω       => l
+               | ⟨r,l'⟩, ⟨s,m'⟩ => match bt_leq r s with 
+                                     | ω => ⟨s,bt_merge_rec n l m'⟩
+                                     | _ => ⟨r,bt_merge_rec n l' m⟩
+                                   end
+             end
+  end.
+
+*)
+
+  Variable (v x1 y1 : Var).
+
+  Definition fe_merge :=
+     MATCH £u WITH
+        ø   ⇒ ø
+     OR u#v ⇒ MATCH £u WITH
+          ø    ⇒ £v
+       OR x#x1 ⇒ MATCH £v WITH
+            ø    ⇒ £u
+         OR y#y1 ⇒ MATCH CALL p_leq ON (£x#£y) WITH
+                ø   ⇒ £y#CALL p_merge ON (£u#£y1)
+             OR u#u ⇒ £x#CALL p_merge ON (£x1#£v).
+
+  Hypothesis (Hparam_merge : param p_merge = u) (Hbody_merg : body p_merge = fe_merge).
+
+  Fact fe_merge_spec f e l m : f // e ~~> ⟨l,m⟩ -> CALL p_merge ON f // e ~~> bt_merge l m.
+  Proof.
+    revert l m.
+    Check measure_rect2.
+    apply measure_rect2 with (m := fun l m => bt_length l+bt_length m).
+ induction on l m as IH with measure (bt_length l+bt_length m).
+
+
+   
+    
+
+
+
+         OR x#x ⇒ ø#ø
+       OR u#x ⇒ MATCH £y WITH
+            ø   ⇒ ø#(ø#ø)
+
+
+           (Hparam_mul : param p_mul = u)
+           (Hparam_fact : param p_fact = u)
+           (Hparam_leb : param p_leb = u)
+           (Hparam_size : param p_size = u) 
+
+           (Hbody_add : body p_add = fe_add) 
+           (Hbody_mul : body p_mul = fe_mul)
+           (Hbody_fact : body p_fact = fe_fact)
+           (Hbody_leb : body p_leb = fe_leb)
+           (Hbody_size : body p_size = fe_size).
+
+
+  Fact f_cmp
+
+  Definition fe_add := 
+    MATCH £u WITH
+         ø   ⇒ ø 
+      OR x#z ⇒ 
+      MATCH £x WITH
+           ø   ⇒ £z 
+        OR x#y ⇒ ø#CALL p_add ON (£y#£z).
+
